add do-while loop lemmas; prove spi_write

bedrock2/src/Examples/SPI.v
@@ -22,12 +22,12 @@ Definition spi_write : function :=
     i = (patience); while (i) { i = (i - constr:(1));
       io! busy = MMIOREAD(SPI_WRITE_ADDR);
       if !(busy >> constr:(31)) {
-        i = (i^i);
-        busy = (busy ^ busy)
+        i = (i^i)
       }
     };
-    if !busy {
-      output! MMIOWRITE(SPI_WRITE_ADDR, b)
+    if !(busy >> constr:(31)) {
+      output! MMIOWRITE(SPI_WRITE_ADDR, b);
+      busy = (busy ^ busy)
     }
   ))).
 
@@ -63,21 +63,138 @@ Require Import bedrock2.ProgramLogic.
 Require Import bedrock2.FE310CSemantics.
 Require Import coqutil.Word.Interface.
 Require Import Coq.Lists.List. Import ListNotations.
-Require Import bedrock2.ReversedListNotations bedrock2.TracePredicate. Import TracePredicateNotations.
-Require Import bedrock2.Examples.lightbulb_spec.
-Fail
-Instance spec_of_spi_write : spec_of "spi_write" := fun functions => forall t m b,
-  WeakestPrecondition.call functions "spi_write" t m [b] (fun T M RETS =>
-    M = m /\ Logic.or
-      ((exists err, word.unsigned err <> 0 /\ RETS = [err]) /\ (eq t +++ (spi_write_full^* )) T)
-      (RETS = [word.of_Z 0] /\ T = t ++ (*FIXME*)nil)).
-(* The term "spi_write_full" has type *)
-(*  "word 8 -> forall word : word 32, list (OP word) -> Prop" *)
-(* while it is expected to have type "list ?T -> Prop". *)
+Require Import bedrock2.TracePredicate. Import TracePredicateNotations.
+Require bedrock2.Examples.lightbulb_spec.
 
-(*
-Require Import coqutil.Map.Interface.
-Lemma spi_write_ok : program_logic_goal_for_function! spi_write.
+Import coqutil.Map.Interface.
+
+Definition mmio_event_abstraction_relation
+  (h : lightbulb_spec.OP Semantics.word)
+  (l : Semantics.mem * Syntax.actname * list Semantics.word * (Semantics.mem * list Semantics.word)) :=
+  Logic.or
+    (exists a v, h = lightbulb_spec.st _ a v /\ l = (map.empty, "MMIOWRITE", [a; v], (map.empty, [])))
+    (exists a v, h = lightbulb_spec.ld _ a v /\ l = (map.empty, "MMIOREAD", [a], (map.empty, [v]))).
+Definition mmio_trace_abstraction_relation := List.Forall2 mmio_event_abstraction_relation.
+
+Import ReversedListNotations.
+Instance spec_of_spi_write : spec_of "spi_write" := fun functions => forall t m b,
+  word.unsigned b < 2 ^ 8 ->
+  WeakestPrecondition.call functions "spi_write" t m [b] (fun T M RETS =>
+    M = m /\ exists iol, T = t ;++ iol /\ exists ioh, mmio_trace_abstraction_relation ioh iol /\ Logic.or
+      ((exists err, RETS = [err] /\ word.unsigned (word.sru err (word.of_Z 31)) <> 0))
+      (RETS = [word.of_Z 0] /\ lightbulb_spec.spi_write Semantics.byte Semantics.word (word.of_Z (word.unsigned b)) ioh)).
+
+Import coqutil.Tactics.letexists.
+Import TailRecursion.
+Lemma spi_write_ok : Semantics.parameters_ok parameters -> program_logic_goal_for_function! spi_write.
 Proof.
+  intros p_ok.
   repeat straightline.
- *)
+  rename H into Hb.
+  show_program.
+
+  (* WHY do theese parentheses matter? *)
+  Fail refine (atleastonce ["b"; "busy"; "i"] (fun v t m b busy i => True) _ _ _ _ _ _ _).
+  refine ((atleastonce ["b"; "busy"; "i"] (fun v T M B BUSY I =>
+     b = B /\
+     v = word.unsigned I /\
+     word.unsigned I <> 0 /\
+     M = m /\
+     exists tl, T = tl++t /\
+     exists th, mmio_trace_abstraction_relation th tl /\
+     lightbulb_spec.spi_write_full _ ^* th))
+          _ _ _ _ _ _ _);
+    cbn [reconstruct map.putmany_of_list HList.tuple.to_list
+         HList.hlist.foralls HList.tuple.foralls
+         HList.hlist.existss HList.tuple.existss
+         HList.hlist.apply  HList.tuple.apply
+         HList.hlist
+         List.repeat Datatypes.length
+         HList.polymorphic_list.repeat HList.polymorphic_list.length
+         PrimitivePair.pair._1 PrimitivePair.pair._2] in *.
+  { repeat straightline. }
+  { eapply (Z.lt_wf 0). }
+  { eexists; split; repeat straightline. inversion H. }
+  { repeat (split; trivial; []).
+    split.
+    { cbv; congruence. }
+    split; trivial.
+    eexists; split.
+    { rewrite app_nil_l; trivial. }
+    eexists; split; constructor. }
+  repeat straightline.
+  eapply WeakestPreconditionProperties.interact_nomem; repeat straightline.
+  split.
+  { cbv. clear. firstorder congruence. }
+  repeat straightline. split; trivial.
+  letexists. split.
+  { repeat straightline. exact eq_refl. }
+  (* evaluate condition then split if *) letexists; split; [solve[repeat straightline]|split].
+  all: repeat (straightline).
+  { do 3 letexists; repeat straightline.
+    eexists; split.
+    { repeat (split; trivial; []). subst t0.
+      eexists (_ ;++ cons _ nil); split; [exact eq_refl|].
+      eexists; split.
+      { refine (List.Forall2_app _ _); try eassumption.
+        econstructor; [|constructor].
+        right; eexists _, _; repeat split. }
+      eapply kleene_app; eauto.
+      refine (kleene_step _ _ nil _ (kleene_empty _)).
+      repeat econstructor.
+      repeat match goal with x:=_|-_=>subst x end.
+      rewrite Properties.word.unsigned_sru_nowrap in H by exact eq_refl; eapply H. }
+    { split; try eapply Properties.word.decrement_nonzero_lt;
+        try eapply Properties.word.unsigned_range; eauto. } }
+  { letexists; split; [solve[repeat straightline]|split]; repeat straightline; try contradiction.
+    split; eauto.
+    subst t0.
+    eexists (_ ;++ cons _ nil); split.
+    { rewrite <-app_assoc; cbn [app]; f_equal. }
+    eexists. split.
+    { eapply Forall2_app; eauto.
+      constructor; [|constructor].
+      right; eauto. }
+    { left; repeat split; eauto. } }
+  { do 3 letexists; repeat straightline.
+    subst i.
+    rewrite Properties.word.unsigned_xor_nowrap in *; rewrite Z.lxor_nilpotent in *; contradiction. }
+  (* evaluate condition then split if *) letexists; split; [solve[repeat straightline]|split].
+  1:contradiction.
+  repeat straightline.
+  eapply WeakestPreconditionProperties.interact_nomem; repeat straightline.
+  split.
+  { cbv. clear. firstorder congruence. }
+  repeat straightline. split; trivial.
+  repeat straightline.
+  split; trivial. subst t0.
+  eexists (_ ;++ cons _ (cons _ nil)). split.
+  { rewrite <-app_assoc. cbn [app]. f_equal. }
+  eexists. split.
+  { eapply List.Forall2_app; eauto.
+    { constructor.
+      { left. eexists _, _; repeat split. }
+      { right; [|constructor].
+        right; eexists _, _; repeat split. } } }
+  right.
+  subst busy.
+  split.
+  { f_equal. eapply Properties.word.unsigned_inj.
+    rewrite Properties.word.unsigned_xor_nowrap; rewrite Z.lxor_nilpotent; reflexivity. }
+  cbv [lightbulb_spec.spi_write].
+  eexists _, _; split; eauto; []; split; eauto.
+  eexists (cons _ nil), (cons _ nil); split; cbn [app]; eauto.
+  split; repeat econstructor.
+  { repeat match goal with x:=_|-_=>subst x end.
+    rewrite Properties.word.unsigned_sru_nowrap in H by exact eq_refl; eapply H. }
+  { cbv [lightbulb_spec.spi_write_enqueue one].
+    repeat f_equal.
+    eapply Properties.word.unsigned_inj.
+    clear -Hb.
+    pose proof Properties.word.unsigned_range b.
+    change (Semantics.width) with 32 in *.
+    do 2 (rewrite word.unsigned_of_Z; cbv [word.wrap]; rewrite Z.mod_small); Lia.lia. }
+  
+  Unshelve.
+  all : intros; exact True.
+Qed.
